nix/ocaml-protoc-plugin.nix
@@ -1,0 +1,51 @@
+{
+  lib,
+  fetchFromGitHub,
+  buildDunePackage,
+  ocaml,
+  pkg-config,
+  protobuf,
+  ocamlPackages,
+  ...
+}: let
+  omd = ocamlPackages.omd.overrideAttrs (final: prev: {
+    version = "2.0.0-alpha4";
+    src = fetchFromGitHub {
+      owner = "ocaml-community";
+      repo = "omd";
+      rev = "373e3f80e48001a62daf4072373ad3aa589ca65f";
+      hash = "sha256-5eZitDaNKSkLOsyPf5g5v9wdZZ3iVQGu8Ot4FHZZ3AI=";
+    };
+    buildInputs = with ocamlPackages; [dune-build-info uucp uunf uutf];
+  });
+in
+  buildDunePackage rec {
+    pname = "ocaml-protoc-plugin";
+    version = "2025-07-09-main";
+
+    minimalOcamlVersion = "4.14";
+
+    src = fetchFromGitHub {
+      owner = "andersfugmann";
+      repo = pname;
+      rev = "27b7eda3c775dc5a140cec0f57bd7e1ba3410152";
+      hash = "sha256-JKhzAZYnXu17v4LGkiXGNH2G5cxnXrPKtfEtZmkGbBw=";
+    };
+
+    checkInputs = with ocamlPackages; [dune-configurator yojson];
+    buildInputs = with ocamlPackages;
+      [
+        base64
+        omd
+        ppx_expect
+        ppx_deriving
+        ptime
+        uucp
+        uunf
+        uutf
+      ]
+      ++ [protobuf];
+    nativeBuildInputs = [pkg-config protobuf];
+
+    doCheck = lib.versionAtLeast ocaml.version "4.14";
+  }
